src/Impl_vm.v
@@ -13,10 +13,10 @@ Fixpoint copland_compile (t:AnnoTerm): CVM unit :=
   | aasp (n,_) a =>
       e <- do_prim n a ;;
       put_ev e
-  | aatt (reqi,rpyi) q t' =>
-      sendReq t' q reqi ;;
-      doRemote t' q reqi rpyi ;;
-      e' <- receiveResp rpyi q ;;
+  | aatt (i,j) (req_loc,rpy_loc) q t' =>
+      sendReq t' q i req_loc ;;
+      doRemote t' q req_loc rpy_loc ;;
+      e' <- receiveResp j rpy_loc q ;;
       put_ev e'
   | alseq r t1 t2 =>
       copland_compile t1 ;;
@@ -33,15 +33,19 @@ Fixpoint copland_compile (t:AnnoTerm): CVM unit :=
       copland_compile t2 ;;
       e2r <- get_ev ;;
       join_seq (Nat.pred y) p e1r e2r
-  | abpar (x,y) (sp1,sp2) t1 t2 =>
+  | abpar (x,y) (loc_e1,loc_e1') (loc_e2,loc_e2') (sp1,sp2) t1 t2 =>
       e <- get_ev ;;
       p <- get_pl ;;
-      pr <- split_ev_par x sp1 sp2 t1 t2 e p ;;
-      let '(loc_e1,loc_e2) := pr in
+      split_ev_par x sp1 sp2 loc_e1 loc_e2 t1 t2 e p ;;
+      (*let '(loc_e1,loc_e2) := pr in*)
       (*let loc_e1 := fst (range t1) in *)
+
+      (*
       let loc_e1' := snd (range t1)  - 1 in  (* TODO: different loc? *)
       (*let loc_e2 := fst (range t2) in *)
       let loc_e2' := snd (range t2) - 1 in   (* TODO: different loc? *)
+       *)
+      
       (*
       let loc_e1 := fst (range t1) in
       let loc_e1' := snd (range t1) - 1 in  (* TODO: different loc? *)
